cleaning

theories/Impure.v
@@ -14,7 +14,7 @@
     <<Program>> monad introduced by the <<operational>> package (see
     <<https://github.com/whitequark/unfork#introduction>>). *)
 
-From mathcomp Require Import ssreflect ssrfun.
+From mathcomp Require Import all_boot boolp.
 From Stdlib Require Import Program Setoid Morphisms.
 From HB Require Import structures.
 From monae Require Import preamble hierarchy.
@@ -40,122 +40,107 @@ Generalizable All Variables.
     to interpret impure computations within Coq, providing an operational
     semantics for [i]. *)
 
-Inductive impure (i : interface) (α : Type) : Type :=
-| local (x : α) : impure i α
-| request_then {β} (e : i β) (f : β -> impure i α) : impure i α.
+Inductive freer (i : effect) (α : Type) : Type :=
+| pure (x : α) : freer i α
+| impure {β} (e : i β) (f : β -> freer i α) : freer i α.
 
-Arguments local [i α] (x).
-Arguments request_then [i α β] (e f).
+Arguments pure [i α] (x).
+Arguments impure [i α β] (e f).
 
-Register impure as freespec.core.impure.type.
-Register local as freespec.core.impure.local.
-Register request_then as freespec.core.impure.request_then.
+Fixpoint freer_bind (i : effect) {α β} (p : freer i α) (f : α -> freer i β)
+    : freer i β :=
+  match p with
+  | pure x => f x
+  | impure Y e g => impure e (fun x => freer_bind (g x) f)
+  end.
 
-Declare Scope impure_scope.
-Bind Scope impure_scope with impure.
-Delimit Scope impure_scope with impure.
-
-HB.mixin Record isMonadImpure (i : interface) (M : UU0 -> UU0) of Monad M := {
-    request : i ~~> M ; 
-    impure_lift (N : monad) (l : i ~~> N) : M ~~> N ;
-    impure_lift_ret : forall (N : monad) (l : i ~~> N) X (x : X),
-        impure_lift N l X (ret X x) = @ret N X x;
-    impure_lift_bind : forall (N : monad) (l : i ~~> N) X Y m (f : X -> M Y), 
-        impure_lift N l Y (m >>= f) = (impure_lift N l X m) >>= (fun x => impure_lift N l Y (f x)) ;
-    impure_lift_request : forall (N : monad) (l : i ~~> N) X (fx : i X), 
-        impure_lift N l X (request X fx) = l X fx;
-    impure_lift_unique : forall (N : monad) (l : i ~~> N) (impure_lift' : M ~~> N),
-            (forall X (x : X), impure_lift' X (ret X x) = @ret N X x) ->
-            (forall X Y (m : M X) (f : X -> M Y), impure_lift' Y (m >>= f) = (impure_lift' X m) >>= (fun x => impure_lift' Y (f x))) ->
-            (forall X (fx : i X), (impure_lift' X (request X fx)) = l X fx) ->
-        forall X (m : M X), impure_lift' X m = impure_lift N l X m
-}.
-
-
-#[short(type=impureMonad)]
-HB.structure Definition MonadImpure (i : interface) := {M of isMonadImpure i M & isMonad M & isFunctor M}.
-
-(** * Monad Instances *)
+Declare Scope freer_scope.
+Bind Scope freer_scope with freer.
+Delimit Scope freer_scope with freer.
 
 (** We then provide the necessary instances of the <<coq-prelude>> Monad
     typeclasses hierarchy. *)
-Module ImpureModule.
+(* mode of the freer monad *)
+Module Monad.
 Section freer.
-
-Variable i : UU0 -> UU0.
-Definition acto := fun X => @impure i X.
+Context (i : UU0 -> UU0).
+Definition acto := @freer i.
 Notation FM := acto.
 
-Definition impure_pure {α} (x : α) : impure i α := local x.
+Let ret : idfun ~~> FM := fun x => @pure i x.
 
-Let ret : idfun ~~> FM := fun _ => impure_pure. 
-
-Fixpoint impure_bind {α β} (p : impure i α) (f : α -> impure i β) : impure i β :=
-  match p with
-  | local x => f x
-  | request_then Y e g => request_then e (fun x => impure_bind (g x) f)
-  end.
-
-Let bind := fun A B m f => @impure_bind A B m f.
+Let bind := fun A B m f => @freer_bind i A B m f.
 
 Let left_neutral : BindLaws.left_neutral bind ret.
-Proof.
-     by [].
-Qed.
+Proof. by []. Qed.
 
 Let right_neutral : BindLaws.right_neutral bind ret.
-Proof.
-    move=>/=A.
-    elim=>[x|Y fy k IHm]//=.
-    congr request_then.
-    exact/boolp.funext=>y.
-Qed.
+Proof. by move=> T; elim => //b e f ih/=; congr impure; exact/funext. Qed.
 
 Let assoc : BindLaws.associative bind.
-Proof.
-    move=>/=A B C m f g.
-    elim:m=>//=Y fy k IHm.
-    congr request_then.
-    exact/boolp.funext=>y.
-Qed.
+Proof. by move=> A B C + f g; elim=>//= *; congr impure; exact/funext. Qed.
 
-HB.instance Definition _ := @isMonad_ret_bind.Build acto ret bind left_neutral right_neutral assoc.
+HB.instance Definition _ := @isMonad_ret_bind.Build acto ret bind
+  left_neutral right_neutral assoc.
 
-(** * Defining Impure Computations *)
+(** * Defining Freer Computations *)
 
-(** FreeSpec users shall not use the [impure] monad constructors directly.  The
+(** FreeSpec users shall not use the [freer] monad constructors directly.  The
     [pure] function from the [Applicative] typeclass allows for defining pure
-    computations which do not depend on any impure primitive.  The [bind]
-    function from the [Monad] typeclass allows for seamlessly combine impure
+    computations which do not depend on any freer primitive.  The [bind]
+    function from the [Monad] typeclass allows for seamlessly combine freer
     computations together.
 
     To complete these two monadic operations, we introduce the [request]
-    function, whose purpose is to define an impure computation that uses a given
+    function, whose purpose is to define an freer computation that uses a given
     primitive [e] from an interface [i], and returns its result.  [request] does
-    not parameterize the [impure] monad with [i] directly, but rather with a
+    not parameterize the [freer] monad with [i] directly, but rather with a
     generic interface [ix].  [ix] is constrained with the [Provide] notation, so
     that it has to provide at least [i]'s primitives.  *)
 
 End freer.
-End ImpureModule.
+End Monad.
 
-HB.export ImpureModule.
+(*HB.export FreerModule.*)
 
-Module Impure.
+HB.mixin Record isMonadFreer (i : effect) (M : UU0 -> UU0) of Monad M := {
+  request : i ~~> M ;
+  denote (N : monad) (l : i ~~> N) : M ~~> N ;
+  denote_ret : forall (N : monad) (l : i ~~> N) X (x : X),
+    denote N l X (ret X x) = @ret N X x ;
+  denote_bind : forall (N : monad) (l : i ~~> N) X Y m (f : X -> M Y),
+    denote N l Y (m >>= f) = denote N l X m >>= (fun x => denote N l Y (f x)) ;
+  denote_request : forall (N : monad) (l : i ~~> N) X (fx : i X),
+    denote N l X (request X fx) = l X fx ;
+  denote_unique : forall (N : monad) (l : i ~~> N) (denote' : M ~~> N),
+      (forall X (x : X), denote' X (ret X x) = @ret N X x) ->
+      (forall X Y (m : M X) (f : X -> M Y), denote' Y (m >>= f) =
+         (denote' X m) >>= (fun x => denote' Y (f x))) ->
+      (forall X (fx : i X), (denote' X (request X fx)) = l X fx) ->
+    forall X (m : M X), denote' X m = denote N l X m
+}.
+
+#[short(type=freerMonad)]
+HB.structure Definition MonadFreer (i : interface) :=
+  {M of isMonadFreer i M & isMonad M & isFunctor M}.
+
+(** * Monad Instances *)
+Module Freer.
 Section freer.
-
 Variable i : interface.
+
+Import Monad.
 
 Local Notation M := (acto i).
 
 Definition requesti : i ~~> acto i := fun α e => 
-  request_then (inj_p e) (fun x => local x).
+  impure (inj_p e) (@pure _ _).
 
 Definition lifter (M : monad) `(l : i ~~> M) : acto i ~~> M :=
   fix aux a (p : acto i a) :=
     match p with
-    | local x => Ret x
-    | request_then Y e f => l _ e >>= fun x => aux a (f x)
+    | pure x => Ret x
+    | impure Y e f => l _ e >>= fun x => aux a (f x)
     end.
 
 Let lifter_ret : forall (cm : monad) (lifter_effect : i ~~> cm) X (x : X),
@@ -177,12 +162,9 @@ Proof.
     exact/boolp.funext/H.
 Qed.
 
-Let lifter_trigger : forall (cm : monad) (lifter_effect : i ~~> cm) X (fx : i X), 
-        lifter lifter_effect (requesti fx) = lifter_effect X fx.
-Proof.
-    move=>cm lifter_effect X fx.
-    by rewrite/lifter/requesti/=bindmret. 
-Qed.
+Let lifter_trigger (cm : monad) (lifter_effect : i ~~> cm) X (fx : i X) :
+  lifter lifter_effect (requesti fx) = lifter_effect X fx.
+Proof. by rewrite /lifter /requesti/= bindmret. Qed.
 
 Let lifter_unique : forall (cm : monad) (lifter_effect : i ~~> cm) (lifter' : M ~~> cm),
             (forall X (x : X), lifter' X (ret X x) = @hierarchy.ret cm X x) ->
@@ -198,29 +180,27 @@ Proof.
     by rewrite -dtrigger'-dbind'/requesti.
 Qed.
 
-HB.instance Definition _ := isMonadImpure.Build i M 
-  lifter_ret 
-  lifter_bind 
-  lifter_trigger
-  lifter_unique.
+HB.instance Definition _ := isMonadFreer.Build i M
+  lifter_ret lifter_bind lifter_trigger lifter_unique.
 
 End freer.
-End Impure.
-HB.export Impure.
+End Freer.
 
-Lemma impure_lift_if : forall (i : interface) (M : impureMonad i) (cm : monad) (lifter_effect : i ~~> cm) X (m m' : M X) b, 
-        impure_lift cm lifter_effect X (if b then m else m') = if b then ( impure_lift cm lifter_effect X m) else ( impure_lift cm lifter_effect X m').
-Proof.
-    by move=>? ? ? ? ? ? ?; case.
-Qed.
-HB.export impure_lift_if.
+Lemma denote_if : forall (i : effect) (M : freerMonad i) (cm : monad)
+   (lifter_effect : i ~~> cm) X (m m' : M X) b,
+  denote cm lifter_effect X (if b then m else m') =
+  if b then (denote cm lifter_effect X m) else (denote cm lifter_effect X m').
+Proof. by move=> ? ? ? ? ? ? ?; case. Qed.
 
+(* example of freer monad using state *)
 Module ImpSt.
-  Section impstate.
-        Variable i : interface.
-        Variable S : UU0.
+Section impstate.
+Context (i : effect) (S : UU0).
+
+Import Monad.
+
 Definition requestis `{Provide ix i} {A} (e : i A): acto ix A :=
-  request_then (inj_p e) (fun x => local x).
+  impure (inj_p e) (@pure _ _).
 
   Let iget `{Provide i (STORE S)} : acto i S:=requestis (inj_p Get).
   Let iput `{Provide i (STORE S)} (s : S) : acto i ():=requestis (inj_p (Put s)).
@@ -229,7 +209,7 @@ Definition requestis `{Provide ix i} {A} (e : i A): acto ix A :=
     function (to seamlessly use [request] with a [MonadTrans] instance such as
     [state_t]). The reason why it has not been kept into the codebase is that
     the flexibility it gives for writing code has a real impact on the
-    verification process. It is simpler to reason about “pure” impure
+    verification process. It is simpler to reason about “pure” freer
     computations (that is, not within a monad stack), then wrapping these
     computations thanks to [lift].
 
@@ -244,10 +224,10 @@ End ImpSt.
 
 (* HB.export ImpSt. *)
 
-Module ImpureFuns.
-Definition trigger  `{Provide ix i} {im : impureMonad ix} : ix ~~> im := fun a e => request a (inj_p e). 
-Definition iget {S} `{Provide i (STORE S)} {im : impureMonad i} : im S:= trigger (inj_p Get).
-Definition iput {S} `{Provide i (STORE S)} {im : impureMonad i} (s : S) : im unit:= trigger (inj_p (Put s)).
-End ImpureFuns.
+Module FreerFuns.
+Definition trigger  `{Provide ix i} {im : freerMonad ix} : ix ~~> im := fun a e => request a (inj_p e). 
+Definition iget {S} `{Provide i (STORE S)} {im : freerMonad i} : im S:= trigger (inj_p Get).
+Definition iput {S} `{Provide i (STORE S)} {im : freerMonad i} (s : S) : im unit:= trigger (inj_p (Put s)).
+End FreerFuns.
 
-HB.export ImpureFuns.
+(*HB.export FreerFuns.*)
