theories/HoareFacts.v
@@ -13,170 +13,167 @@ Local Open Scope monae_scope.
 
 (** * Primitive Request Views *)
 
-Lemma interface_to_hoare_preE `{MayProvide ix i} `(c : contract i Ω)
-    `(e : ix a) (ω : Ω) :
+Section tmp.
+Context `{MayProvide ix i} `(c : contract i Ω).
+
+Lemma interface_to_hoare_preE `(e : ix a) (ω : Ω) :
   pre (interface_to_hoare c e) ω <-> gen_caller_obligation c ω e.
 Proof. by split. Qed.
 
-Lemma interface_to_hoare_postE `{MayProvide ix i} `(c : contract i Ω)
-    `(e : ix a) (ω : Ω) (x : a) (ω' : Ω) :
+Lemma interface_to_hoare_postE `(e : ix a) (ω : Ω) (x : a) (ω' : Ω) :
   post (interface_to_hoare c e) ω x ω' <->
   gen_callee_obligation c ω e x /\
   ω' = gen_witness_update c ω e x.
 Proof. by split. Qed.
 
-Lemma interface_to_hoare_postI `{MayProvide ix i} `(c : contract i Ω)
-    `(e : ix a) (ω : Ω) (x : a) :
+Lemma interface_to_hoare_postI `(e : ix a) (ω : Ω) (x : a) :
   gen_callee_obligation c ω e x ->
-  post (interface_to_hoare c e) ω x
-       (gen_witness_update c ω e x).
+  post (interface_to_hoare c e) ω x (gen_witness_update c ω e x).
 Proof. by move=> step; split. Qed.
 
-Lemma to_hoare_requestE `{MayProvide ix i} {im : impureMonad ix}
-    `(c : contract i Ω) `(e : ix a) :
-  to_hoare (im:=im) c (request a e) = interface_to_hoare c e.
-Proof. exact: impure_lift_request. Qed.
+Lemma to_hoare_localE `(x : a) :
+  to_hoare (im:=Freer.Monad_acto__canonical__Impure_MonadFreer ix) c (pure x : freer ix a) =
+  Ret x.
+Proof. exact: denote_ret. Qed.
 
-Lemma to_hoare_request_preE `{MayProvide ix i} {im : impureMonad ix}
-    `(c : contract i Ω) `(e : ix a) (ω : Ω) :
+Lemma to_hoare_local_preE `(x : a) (ω : Ω) :
+  pre (to_hoare (im:=Freer.Monad_acto__canonical__Impure_MonadFreer ix)
+                c (pure x : freer ix a)) ω.
+Proof. by rewrite to_hoare_localE hoare_pure_preE. Qed.
+
+Lemma to_hoare_bindE `(p : freer ix a) `(f : a -> freer ix b) :
+  to_hoare (im:=Freer.Monad_acto__canonical__Impure_MonadFreer ix)
+           c (freer_bind p f) =
+  to_hoare (im:=Freer.Monad_acto__canonical__Impure_MonadFreer ix) c p
+    >>= fun x =>
+      to_hoare (im:=Freer.Monad_acto__canonical__Impure_MonadFreer ix)
+               c (f x).
+Proof. exact: denote_bind. Qed.
+
+Lemma to_hoare_bind_preE `(p : freer ix a) `(f : a -> freer ix b) (ω : Ω) :
+  pre (to_hoare (im:=Freer.Monad_acto__canonical__Impure_MonadFreer ix)
+                c (freer_bind p f)) ω <->
+  pre (to_hoare (im:=Freer.Monad_acto__canonical__Impure_MonadFreer ix)
+                c p) ω /\
+  forall x ω',
+    post (to_hoare
+            (im:=Freer.Monad_acto__canonical__Impure_MonadFreer ix)
+            c p) ω x ω' ->
+    pre (to_hoare
+           (im:=Freer.Monad_acto__canonical__Impure_MonadFreer ix)
+           c (f x)) ω'.
+Proof. by rewrite to_hoare_bindE hoare_bind_preE. Qed.
+
+Lemma to_hoare_bind_preI `(p : freer ix a) `(f : a -> freer ix b) (ω : Ω) :
+  pre (to_hoare (im:=Freer.Monad_acto__canonical__Impure_MonadFreer ix)
+                c p) ω ->
+  (forall x ω',
+    post (to_hoare
+            (im:=Freer.Monad_acto__canonical__Impure_MonadFreer ix)
+            c p) ω x ω' ->
+    pre (to_hoare
+           (im:=Freer.Monad_acto__canonical__Impure_MonadFreer ix)
+           c (f x)) ω') ->
+  pre (to_hoare (im:=Freer.Monad_acto__canonical__Impure_MonadFreer ix)
+                c (freer_bind p f)) ω.
+Proof. by move=> prefix suffix; apply/to_hoare_bind_preE; split. Qed.
+
+End tmp.
+
+Section tmp.
+Context `{MayProvide ix i} {im : freerMonad ix} `(c : contract i Ω).
+
+Lemma to_hoare_requestE `(e : ix a) :
+  to_hoare (im:=im) c (request a e) = interface_to_hoare c e.
+Proof. exact: denote_request. Qed.
+
+Lemma to_hoare_request_preE `(e : ix a) (ω : Ω) :
   pre (to_hoare (im:=im) c (request a e)) ω <->
   gen_caller_obligation c ω e.
 Proof. by rewrite to_hoare_requestE interface_to_hoare_preE. Qed.
 
-Lemma to_hoare_request_postE `{MayProvide ix i} {im : impureMonad ix}
-    `(c : contract i Ω) `(e : ix a) (ω : Ω) (x : a) (ω' : Ω) :
+Lemma to_hoare_request_postE `(e : ix a) (ω : Ω) (x : a) (ω' : Ω) :
   post (to_hoare (im:=im) c (request a e)) ω x ω' <->
   gen_callee_obligation c ω e x /\
   ω' = gen_witness_update c ω e x.
 Proof. by rewrite to_hoare_requestE interface_to_hoare_postE. Qed.
 
-Lemma to_hoare_request_postI `{MayProvide ix i} {im : impureMonad ix}
-    `(c : contract i Ω) `(e : ix a) (ω : Ω) (x : a) :
+Lemma to_hoare_request_postI `(e : ix a) (ω : Ω) (x : a) :
   gen_callee_obligation c ω e x ->
   post (to_hoare (im:=im) c (request a e)) ω x
        (gen_witness_update c ω e x).
 Proof. by rewrite to_hoare_requestE; exact: interface_to_hoare_postI. Qed.
 
-(** * Canonical Impure Views *)
-
-Lemma to_hoare_localE `{MayProvide ix i} `(c : contract i Ω) `(x : a) :
-  to_hoare
-    (im:=ImpureModule_acto__canonical__Impure_MonadImpure ix)
-    c (local x : impure ix a) = Ret x.
-Proof. exact: impure_lift_ret. Qed.
-
-Lemma to_hoare_local_preE `{MayProvide ix i} `(c : contract i Ω)
-    `(x : a) (ω : Ω) :
-  pre (to_hoare (im:=ImpureModule_acto__canonical__Impure_MonadImpure ix)
-                c (local x : impure ix a)) ω <-> True.
-Proof. by rewrite to_hoare_localE hoare_pure_preE. Qed.
-
-Lemma to_hoare_local_preI `{MayProvide ix i} `(c : contract i Ω)
-    `(x : a) (ω : Ω) :
-  pre (to_hoare (im:=ImpureModule_acto__canonical__Impure_MonadImpure ix)
-                c (local x : impure ix a)) ω.
+Lemma to_hoare_local_preI `(x : a) (ω : Ω) :
+  pre (to_hoare (im:=Freer.Monad_acto__canonical__Impure_MonadFreer ix)
+                c (pure x : freer ix a)) ω.
 Proof. by apply/to_hoare_local_preE. Qed.
 
-Lemma to_hoare_local_postE `{MayProvide ix i} `(c : contract i Ω)
-    `(x : a) (y : a) (ω ω' : Ω) :
-  post (to_hoare (im:=ImpureModule_acto__canonical__Impure_MonadImpure ix)
-                 c (local x : impure ix a)) ω y ω' <->
+Lemma to_hoare_local_postE `(x : a) (y : a) (ω ω' : Ω) :
+  post (to_hoare (im:=Freer.Monad_acto__canonical__Impure_MonadFreer ix)
+                 c (pure x : freer ix a)) ω y ω' <->
   x = y /\ ω = ω'.
 Proof. by rewrite to_hoare_localE hoare_pure_postE. Qed.
 
-Lemma to_hoare_local_postI `{MayProvide ix i} `(c : contract i Ω)
-    `(x : a) (ω : Ω) :
-  post (to_hoare (im:=ImpureModule_acto__canonical__Impure_MonadImpure ix)
-                 c (local x : impure ix a)) ω x ω.
+Lemma to_hoare_local_postI `(x : a) (ω : Ω) :
+  post (to_hoare (im:=Freer.Monad_acto__canonical__Impure_MonadFreer ix)
+                 c (pure x : freer ix a)) ω x ω.
 Proof. by apply/to_hoare_local_postE; split. Qed.
 
-Lemma to_hoare_bindE `{MayProvide ix i} `(c : contract i Ω)
-    `(p : impure ix a) `(f : a -> impure ix b) :
-  to_hoare (im:=ImpureModule_acto__canonical__Impure_MonadImpure ix)
-           c (impure_bind p f) =
-  to_hoare (im:=ImpureModule_acto__canonical__Impure_MonadImpure ix) c p
-    >>= fun x =>
-      to_hoare (im:=ImpureModule_acto__canonical__Impure_MonadImpure ix)
-               c (f x).
-Proof. exact: impure_lift_bind. Qed.
+End tmp.
 
-Lemma to_hoare_bind_preE `{MayProvide ix i} `(c : contract i Ω)
-    `(p : impure ix a) `(f : a -> impure ix b) (ω : Ω) :
-  pre (to_hoare (im:=ImpureModule_acto__canonical__Impure_MonadImpure ix)
-                c (impure_bind p f)) ω <->
-  pre (to_hoare (im:=ImpureModule_acto__canonical__Impure_MonadImpure ix)
-                c p) ω /\
-  forall x ω',
-    post (to_hoare
-            (im:=ImpureModule_acto__canonical__Impure_MonadImpure ix)
-            c p) ω x ω' ->
-    pre (to_hoare
-           (im:=ImpureModule_acto__canonical__Impure_MonadImpure ix)
-           c (f x)) ω'.
-Proof. by rewrite to_hoare_bindE hoare_bind_preE. Qed.
+(** * Canonical Impure Views *)
 
-Lemma to_hoare_bind_preI `{MayProvide ix i} `(c : contract i Ω)
-    `(p : impure ix a) `(f : a -> impure ix b) (ω : Ω) :
-  pre (to_hoare (im:=ImpureModule_acto__canonical__Impure_MonadImpure ix)
-                c p) ω ->
-  (forall x ω',
-    post (to_hoare
-            (im:=ImpureModule_acto__canonical__Impure_MonadImpure ix)
-            c p) ω x ω' ->
-    pre (to_hoare
-           (im:=ImpureModule_acto__canonical__Impure_MonadImpure ix)
-           c (f x)) ω') ->
-  pre (to_hoare (im:=ImpureModule_acto__canonical__Impure_MonadImpure ix)
-                c (impure_bind p f)) ω.
-Proof. by move=> prefix suffix; apply/to_hoare_bind_preE; split. Qed.
+Section tmp.
+Context `{MayProvide ix i} `(c : contract i Ω)
+    `(p : freer ix a) `(f : a -> freer ix b).
 
-Lemma to_hoare_bind_postE `{MayProvide ix i} `(c : contract i Ω)
-    `(p : impure ix a) `(f : a -> impure ix b)
-    (ω : Ω) (y : b) (ω' : Ω) :
-  post (to_hoare (im:=ImpureModule_acto__canonical__Impure_MonadImpure ix)
-                 c (impure_bind p f)) ω y ω' <->
+Lemma to_hoare_bind_postE (ω : Ω) (y : b) (ω' : Ω) :
+  post (to_hoare (im:=Freer.Monad_acto__canonical__Impure_MonadFreer ix)
+                 c (freer_bind p f)) ω y ω' <->
   exists x ω'',
     post (to_hoare
-            (im:=ImpureModule_acto__canonical__Impure_MonadImpure ix)
+            (im:=Freer.Monad_acto__canonical__Impure_MonadFreer ix)
             c p) ω x ω'' /\
     post (to_hoare
-            (im:=ImpureModule_acto__canonical__Impure_MonadImpure ix)
+            (im:=Freer.Monad_acto__canonical__Impure_MonadFreer ix)
             c (f x)) ω'' y ω'.
 Proof. by rewrite to_hoare_bindE hoare_bind_postE. Qed.
 
-Lemma to_hoare_bind_postI `{MayProvide ix i} `(c : contract i Ω)
-    `(p : impure ix a) `(f : a -> impure ix b)
+Lemma to_hoare_bind_postI
     (ω : Ω) (x : a) (ω'' : Ω) (y : b) (ω' : Ω) :
-  post (to_hoare (im:=ImpureModule_acto__canonical__Impure_MonadImpure ix)
+  post (to_hoare (im:=Freer.Monad_acto__canonical__Impure_MonadFreer ix)
                  c p) ω x ω'' ->
-  post (to_hoare (im:=ImpureModule_acto__canonical__Impure_MonadImpure ix)
+  post (to_hoare (im:=Freer.Monad_acto__canonical__Impure_MonadFreer ix)
                  c (f x)) ω'' y ω' ->
-  post (to_hoare (im:=ImpureModule_acto__canonical__Impure_MonadImpure ix)
-                 c (impure_bind p f)) ω y ω'.
+  post (to_hoare (im:=Freer.Monad_acto__canonical__Impure_MonadFreer ix)
+                 c (freer_bind p f)) ω y ω'.
 Proof.
 move=> prefix suffix; apply/to_hoare_bind_postE.
 by exists x, ω''.
 Qed.
 
-Lemma to_hoare_request_then_preE `{MayProvide ix i} `(c : contract i Ω)
-    `(e : ix a) `(f : a -> impure ix b) (ω : Ω) :
-  pre (to_hoare (im:=ImpureModule_acto__canonical__Impure_MonadImpure ix)
-                c (request_then e f)) ω <->
+End tmp.
+
+Lemma to_hoare_impure_preE `{MayProvide ix i} `(c : contract i Ω)
+    `(e : ix a) `(f : a -> freer ix b) (ω : Ω) :
+  pre (to_hoare (im:=Freer.Monad_acto__canonical__Impure_MonadFreer ix)
+                c (impure e f)) ω <->
   gen_caller_obligation c ω e /\
   forall x, gen_callee_obligation c ω e x ->
-    pre (to_hoare (im:=ImpureModule_acto__canonical__Impure_MonadImpure ix)
+    pre (to_hoare (im:=Freer.Monad_acto__canonical__Impure_MonadFreer ix)
                   c (f x)) (gen_witness_update c ω e x).
 Proof.
 change
   (pre (interface_to_hoare c e >>=
           fun x =>
             to_hoare
-              (im:=ImpureModule_acto__canonical__Impure_MonadImpure ix)
+              (im:=Freer.Monad_acto__canonical__Impure_MonadFreer ix)
               c (f x)) ω <->
    gen_caller_obligation c ω e /\
    forall x, gen_callee_obligation c ω e x ->
      pre (to_hoare
-            (im:=ImpureModule_acto__canonical__Impure_MonadImpure ix)
+            (im:=Freer.Monad_acto__canonical__Impure_MonadFreer ix)
             c (f x)) (gen_witness_update c ω e x)).
 split.
 - move=> /hoare_bind_preE [caller next]; split.
@@ -189,33 +186,33 @@ move=> x ω' /interface_to_hoare_postE [callee ->].
 exact: next.
 Qed.
 
-Lemma to_hoare_request_then_preI `{MayProvide ix i} `(c : contract i Ω)
-    `(e : ix a) `(f : a -> impure ix b) (ω : Ω) :
+Lemma to_hoare_impure_preI `{MayProvide ix i} `(c : contract i Ω)
+    `(e : ix a) `(f : a -> freer ix b) (ω : Ω) :
   gen_caller_obligation c ω e ->
   (forall x, gen_callee_obligation c ω e x ->
-    pre (to_hoare (im:=ImpureModule_acto__canonical__Impure_MonadImpure ix)
+    pre (to_hoare (im:=Freer.Monad_acto__canonical__Impure_MonadFreer ix)
                   c (f x)) (gen_witness_update c ω e x)) ->
-  pre (to_hoare (im:=ImpureModule_acto__canonical__Impure_MonadImpure ix)
-                c (request_then e f)) ω.
-Proof. by move=> caller next; apply/to_hoare_request_then_preE; split. Qed.
+  pre (to_hoare (im:=Freer.Monad_acto__canonical__Impure_MonadFreer ix)
+                c (impure e f)) ω.
+Proof. by move=> caller next; apply/to_hoare_impure_preE; split. Qed.
 
-Lemma to_hoare_request_then_postE `{MayProvide ix i} `(c : contract i Ω)
-    `(e : ix a) `(f : a -> impure ix b) (ω : Ω) (y : b) (ω' : Ω) :
-  post (to_hoare (im:=ImpureModule_acto__canonical__Impure_MonadImpure ix)
-                 c (request_then e f)) ω y ω' <->
+Lemma to_hoare_impure_postE `{MayProvide ix i} `(c : contract i Ω)
+    `(e : ix a) `(f : a -> freer ix b) (ω : Ω) (y : b) (ω' : Ω) :
+  post (to_hoare (im:=Freer.Monad_acto__canonical__Impure_MonadFreer ix)
+                 c (impure e f)) ω y ω' <->
   exists x, gen_callee_obligation c ω e x /\
-    post (to_hoare (im:=ImpureModule_acto__canonical__Impure_MonadImpure ix)
+    post (to_hoare (im:=Freer.Monad_acto__canonical__Impure_MonadFreer ix)
                    c (f x)) (gen_witness_update c ω e x) y ω'.
 Proof.
 change
   (post (interface_to_hoare c e >>=
            fun x =>
              to_hoare
-               (im:=ImpureModule_acto__canonical__Impure_MonadImpure ix)
+               (im:=Freer.Monad_acto__canonical__Impure_MonadFreer ix)
                c (f x)) ω y ω' <->
    exists x, gen_callee_obligation c ω e x /\
      post (to_hoare
-             (im:=ImpureModule_acto__canonical__Impure_MonadImpure ix)
+             (im:=Freer.Monad_acto__canonical__Impure_MonadFreer ix)
              c (f x)) (gen_witness_update c ω e x) y ω').
 split.
 - move=> /hoare_bind_postE [x [ω'' [step suffix]]].
@@ -229,53 +226,53 @@ Qed.
 (** * General Lemmas *)
 
 Lemma to_hoare_step `{MayProvide ix i} `(c : contract i Ω)
-    `(e : ix a) `(f : a -> impure ix a)
+    `(e : ix a) `(f : a -> freer ix a)
     `(hpre : pre (to_hoare
-      (im:=ImpureModule_acto__canonical__Impure_MonadImpure ix)
-      c (request_then e f)) ω)
+      (im:=Freer.Monad_acto__canonical__Impure_MonadFreer ix)
+      c (impure e f)) ω)
     (x : a) (step : gen_callee_obligation c ω e x) :
   pre (to_hoare
-         (im:=ImpureModule_acto__canonical__Impure_MonadImpure ix)
+         (im:=Freer.Monad_acto__canonical__Impure_MonadFreer ix)
          c (f x)) (gen_witness_update c ω e x).
 
 Proof.
-move: hpre => /to_hoare_request_then_preE [_ next].
+move: hpre => /to_hoare_impure_preE [_ next].
 exact: next.
 Qed.
 
 #[global] Hint Resolve to_hoare_step : freespec.
 
 Lemma to_hoare_pre_bind_assoc `{MayProvide ix i} `(c : contract i Ω)
-    `(p : impure ix a)
+    `(p : freer ix a)
     `(Hp : pre (to_hoare
-      (im:=ImpureModule_acto__canonical__Impure_MonadImpure ix) c p) ω)
-    `(f : a -> impure ix b)
+      (im:=Freer.Monad_acto__canonical__Impure_MonadFreer ix) c p) ω)
+    `(f : a -> freer ix b)
     (run : forall (x : a) (ω' : Ω),
       post (to_hoare
-        (im:=ImpureModule_acto__canonical__Impure_MonadImpure ix)
+        (im:=Freer.Monad_acto__canonical__Impure_MonadFreer ix)
         c p) ω x ω' ->
       pre (to_hoare
-        (im:=ImpureModule_acto__canonical__Impure_MonadImpure ix)
+        (im:=Freer.Monad_acto__canonical__Impure_MonadFreer ix)
         c (f x)) ω') :
   pre (to_hoare
-         (im:=ImpureModule_acto__canonical__Impure_MonadImpure ix)
-         c (impure_bind p f)) ω.
+         (im:=Freer.Monad_acto__canonical__Impure_MonadFreer ix)
+         c (freer_bind p f)) ω.
 
 Proof.
 by apply/to_hoare_bind_preI.
 Qed.
 
 Lemma to_hoare_post_bind_assoc `{MayProvide ix i} `(c : contract i Ω)
-    `(p : impure ix a) `(f : a -> impure ix b)
+    `(p : freer ix a) `(f : a -> freer ix b)
     `(Hp : post (to_hoare
-      (im:=ImpureModule_acto__canonical__Impure_MonadImpure ix)
-      c (impure_bind p f)) ω x ω') :
+      (im:=Freer.Monad_acto__canonical__Impure_MonadFreer ix)
+      c (freer_bind p f)) ω x ω') :
   exists y ω'',
     post (to_hoare
-      (im:=ImpureModule_acto__canonical__Impure_MonadImpure ix)
+      (im:=Freer.Monad_acto__canonical__Impure_MonadFreer ix)
       c p) ω y ω'' /\
     post (to_hoare
-      (im:=ImpureModule_acto__canonical__Impure_MonadImpure ix)
+      (im:=Freer.Monad_acto__canonical__Impure_MonadFreer ix)
       c (f y)) ω'' x ω'.
 
 Proof.
@@ -308,20 +305,20 @@ Proof. by []. Qed.
 
 Lemma to_hoare_contractprod_preI `{Provide ix i, Provide ix j}
     `(ci : contract i Ωi) `(cj : contract j Ωj)
-    `(p : impure ix a) (ωi : Ωi) (ωj : Ωj) :
-  pre (to_hoare (im:=ImpureModule_acto__canonical__Impure_MonadImpure ix)
+    `(p : freer ix a) (ωi : Ωi) (ωj : Ωj) :
+  pre (to_hoare (im:=Freer.Monad_acto__canonical__Impure_MonadFreer ix)
                 ci p) ωi ->
-  pre (to_hoare (im:=ImpureModule_acto__canonical__Impure_MonadImpure ix)
+  pre (to_hoare (im:=Freer.Monad_acto__canonical__Impure_MonadFreer ix)
                 cj p) ωj ->
-  pre (to_hoare (im:=ImpureModule_acto__canonical__Impure_MonadImpure ix)
+  pre (to_hoare (im:=Freer.Monad_acto__canonical__Impure_MonadFreer ix)
                 (ci * cj) p) (ωi, ωj).
 Proof.
 move: p ωi ωj.
 elim=> [x | b e f ih] ωi ωj.
 - by move=> _ _; apply/to_hoare_local_preE.
-move=> /to_hoare_request_then_preE [calleri nexti].
-move=> /to_hoare_request_then_preE [callerj nextj].
-apply/to_hoare_request_then_preI.
+move=> /to_hoare_impure_preE [calleri nexti].
+move=> /to_hoare_impure_preE [callerj nextj].
+apply/to_hoare_impure_preI.
   by apply/contractprod_callerE; split.
 move=> x /contractprod_calleeE [calleei calleej].
 rewrite contractprod_witnessE.
@@ -332,23 +329,23 @@ Qed.
 
 Lemma to_hoare_contractprod `{Provide ix i, Provide ix j}
     `(ci : contract i Ωi) `(cj : contract j Ωj)
-    `(p : impure ix a) `(prei : pre (to_hoare
-      (im:=ImpureModule_acto__canonical__Impure_MonadImpure ix) ci p) ωi)
+    `(p : freer ix a) `(prei : pre (to_hoare
+      (im:=Freer.Monad_acto__canonical__Impure_MonadFreer ix) ci p) ωi)
     `(prej : pre (to_hoare
-      (im:=ImpureModule_acto__canonical__Impure_MonadImpure ix) cj p) ωj) :
-  pre (to_hoare (im:=ImpureModule_acto__canonical__Impure_MonadImpure ix)
+      (im:=Freer.Monad_acto__canonical__Impure_MonadFreer ix) cj p) ωj) :
+  pre (to_hoare (im:=Freer.Monad_acto__canonical__Impure_MonadFreer ix)
                 (ci * cj) p) (ωi, ωj).
 Proof. exact: to_hoare_contractprod_preI prei prej. Qed.
 
 #[global] Hint Resolve to_hoare_contractprod_preI : freespec.
 
 Lemma contract_equ_pre `(c1 : contract i Ω1) `(c2 : contract i Ω2)
-    `(equ : contract_equ c1 c2) (ω1 : Ω1) `(p : impure i A) :
+    `(equ : contract_equ c1 c2) (ω1 : Ω1) `(p : freer i A) :
   pre (to_hoare
-         (im:=ImpureModule_acto__canonical__Impure_MonadImpure i)
+         (im:=Freer.Monad_acto__canonical__Impure_MonadFreer i)
          c1 p) ω1 <->
   pre (to_hoare
-         (im:=ImpureModule_acto__canonical__Impure_MonadImpure i)
+         (im:=Freer.Monad_acto__canonical__Impure_MonadFreer i)
          c2 p) (contract_iso_lr equ ω1).
 
 Proof.
@@ -371,12 +368,12 @@ Qed.
 
 Lemma contract_equ_post `(c1 : contract i Ω1) `(c2 : contract i Ω2)
     `(equ : contract_equ c1 c2) (ω1 ω1' : Ω1)
-    `(p : impure i A) (x : A)
+    `(p : freer i A) (x : A)
     (post1 : post (to_hoare
-      (im:=ImpureModule_acto__canonical__Impure_MonadImpure i)
+      (im:=Freer.Monad_acto__canonical__Impure_MonadFreer i)
       c1 p) ω1 x ω1') :
   post (to_hoare
-          (im:=ImpureModule_acto__canonical__Impure_MonadImpure i)
+          (im:=Freer.Monad_acto__canonical__Impure_MonadFreer i)
           c2 p) (contract_iso_lr equ ω1) x
        (contract_iso_lr equ ω1').
 
